theories/BlockFusionDenotation.v
@@ -1,0 +1,211 @@
+(** This file contains the proof of correctness of the Conditional Constant Propagation optimization.
+    It relies on the garantees given by the [BlockFusion] pattern and on proofs form the [Denotation] file. *)
+
+From Vellvm Require Import Syntax ScopeTheory Semantics Theory Tactics Denotation DenotationTheory.
+From ITree Require Import ITree Eq HeterogeneousRelations.
+From Pattern Require Import Base Patterns Denotation BlockFusion.
+From Paco Require Import paco.
+From stdpp Require Import prelude fin_maps strings.
+Import List Head Focus Block Patterns gmap Utils.Monads PostConditions Pattern.Denotation.
+
+(** [promote_phis] doesn't work at this level because of the interpretation differences between simultaneous phi-nodes and affectation instructions.
+    It is kept to simplify the proof strucutre. *)
+
+Definition promote_phi (idA : block_id) (Φ : local_id * phi dtyp) : option (instr_id * instr dtyp) :=
+  match Φ with
+  | (x, (Phi _ args)) =>
+      match args !! idA with
+      | None => None
+      | Some e => Some (IId x, INSTR_Op e)
+      end end.
+
+Definition promote_phis (idA : block_id) (Φs : list (local_id * phi dtyp)) : code dtyp :=
+  fold_left
+    (fun acc φ => match promote_phi idA φ with
+               | None => acc
+               | Some i => acc ++ [i]
+               end)
+    Φs [].
+
+Definition fusion_code (idA : block_id) (A B: blk): code dtyp :=
+  A.(blk_code) ++ promote_phis idA B.(blk_phis) ++ B.(blk_code).
+
+Definition fusion_comments (A B: blk) :=
+  match (A.(blk_comments), B.(blk_comments)) with
+    | (Some cA, Some cB) => Some (cA++cB)
+    | (Some cA, _) => Some cA
+    | (_, Some cB) => Some cB
+    | (_, _) => None
+  end.
+
+Definition fusion (σ: bid_renaming) (idA : block_id) (A B: blk): blk := {|
+  blk_phis       := A.(blk_phis);
+  blk_code       := fusion_code idA A B;
+  blk_term       := term_rename σ B.(blk_term);
+  blk_comments   := fusion_comments A B
+|}.
+
+Definition σfusion idA idB := fun (id: bid) => if decide (id=idA) then idB else id.
+
+Module Type Theory (LP : LLVMParams.LLVMParams).
+Module DE := Denotation.Make LP.
+Import DE.
+Import DT.
+Import DT.D.
+Import LP.
+Import SemNotations.
+Import MonadNotation.
+Import Events.DV.
+
+Variant hidden_cfg  (T: Type) : Type := boxh_cfg (t: T).
+Variant visible_cfg (T: Type) : Type := boxv_cfg (t: T).
+Ltac hide_cfg :=
+  match goal with
+  | h : visible_cfg _ |- _ =>
+      let EQ := fresh "VG" in
+      destruct h as [EQ];
+      apply boxh_cfg in EQ
+  | |- context[denote_ocfg ?cfg _] =>
+      remember cfg as G eqn:VG;
+      apply boxh_cfg in VG
+  end.
+Ltac show_cfg :=
+  match goal with
+  | h: hidden_cfg _ |- _ =>
+      let EQ := fresh "HG" in
+      destruct h as [EQ];
+      apply boxv_cfg in EQ
+  end.
+Notation "'hidden' G" := (hidden_cfg (G = _)) (only printing, at level 10).
+
+
+Module eutt_Notations.
+  Notation "t '======================' '======================' u '======================' '{' R '}'"
+    := (eutt R t u)
+        (only printing, at level 200,
+          format "'//' '//' t '//' '======================' '======================' '//' u '//' '======================' '//' '{' R '}'"
+        ).
+End eutt_Notations.
+Import eutt_Notations.
+
+Lemma fusion_correct {S} G idA A idB B P (X:S):
+  let σ := σfusion idA idB in
+  (idA, A, (idB, B, X)) ∈ (MatchAll (BlockFusion P) G) ->
+  denote_ocfg_equiv_cond {[idA := A; idB := B]} {[idB := fusion σ idA A B]} {[idA]} {[idB]} σ.
+Proof.
+  intros σ IN. apply Pattern_BlockFusion_correct in IN as (G' & _ & FUS); auto.
+  destruct FUS as [EQ NEQAB LUA LUB PRED SUCC PHI].
+  unfold denote_ocfg_equiv_cond.
+  einit.
+  ecofix cih.
+  clear cihH.
+  intros * NINh NINo.
+  apply not_elem_of_singleton in NINh, NINo.
+  case (decide (header = idA)) as [->|NEQ].
+
+  - subst σ. unfold σfusion.
+    case_match; try done.
+    simplify_eq.
+    rewrite ?denote_ocfg_in_eq_itree; try by simplify_map_eq.
+    destruct A as [phisA codeA termA cA].
+    remember {| blk_phis := phisA; blk_code := codeA; blk_term := termA; blk_comments := cA |} as A.
+    Arguments denote_code : simpl never.
+    Arguments denote_phis : simpl never.
+    Arguments promote_phis : simpl never.
+    Opaque denote_phis.
+    Opaque denote_code.
+
+    cbn. unfold fusion_code.
+    setoid_rewrite bind_bind.
+    ebind. econstructor; [reflexivity|]. intros [] ? <-.
+    setoid_rewrite bind_bind.
+    rewrite denote_code_app_eq_itree.
+    setoid_rewrite bind_bind.
+    ebind. econstructor; [reflexivity|]. intros [] ? <-.
+    cbn in SUCC. rewrite SUCC. cbn. rewrite bind_ret_l.
+    rewrite tau_euttge.
+    rewrite ?denote_ocfg_in_eq_itree; try by simplify_map_eq.
+    destruct B as [phisB codeB termB cB].
+    remember {| blk_phis := phisB; blk_code := codeB; blk_term := termB; blk_comments := cB |} as B.
+    cbn in *.
+    setoid_rewrite bind_bind.
+    rewrite denote_code_app_eq_itree.
+    setoid_rewrite bind_bind.
+    ebind. econstructor.
+    rewrite !PHI. unfold promote_phis. cbn. rewrite denote_phis_nil. rewrite denote_code_nil. reflexivity.
+    intros [] ? <-.
+    ebind. econstructor. reflexivity. intros [] ? <-.
+    ebind. econstructor. eapply has_post_enrich_eutt; [ | | apply term_rename_eutt].
+    apply denote_terminator_exits_in_outputs.
+    apply denote_terminator_exits_in_outputs.
+    intros [] [] (REL1 & REL2 & REL3); inversion REL3.
+    * etau. rewrite <- H2. ebase. right. apply cihL.
+      + apply not_elem_of_singleton. intro EQb. 
+        subst b a1 a2. case_match. now subst. subst b0.
+        assert (BIN: idB ∈ successors B). {
+          inversion REL1. unfold successors. apply H2.
+        }
+        pose proof predecessors_elem_of G _ LUB BIN.
+        rewrite PRED in H1. set_solver.
+      + now apply not_elem_of_singleton.
+    * eret. now subst.
+
+  - assert (EQσ: σ header = header). {
+      subst σ. unfold σfusion. case_match. now subst. reflexivity.
+    } rewrite EQσ.
+    rewrite denote_ocfg_nin_eq_itree; [|now simplify_map_eq].
+    rewrite denote_ocfg_nin_eq_itree; [|now simplify_map_eq].
+    eret.
+Qed.
+
+Theorem Denotation_BlockFusion_correct {S} G idA A idB B f to P (X:S):
+  let σ := σfusion idA idB in
+  let G0 := delete idB (delete idA G) in
+  to <> idB ->
+  f <> idA ->
+  (idA, A, (idB, B, X)) ∈ (MatchAll (BlockFusion P) G) ->
+  ⟦ G ⟧bs (f, to) ≈ ⟦ <[idB:=fusion σ idA A B]> (ocfg_term_rename σ G0) ⟧bs (f, σ to).
+Proof.
+  intros * ineq1 ineq2 IN.
+  apply Pattern_BlockFusion_correct in IN as (G' & INX & FUS); auto.
+  destruct FUS as [EQ LUA LUB PRED SUCC].
+  assert (G0 = G') as -> by now subst G0 G'.
+  assert (BNIN: idB ∉ outputs G'). {
+    unfold outputs. intros H. apply elem_of_fold_bk_acc in H as (id & bk & H1 & H2).
+    unfold outputs_acc in H2. simplify_map_eq.
+    apply lookup_delete_Some in H1 as [? H1]. apply lookup_delete_Some in H1 as [? H1]. 
+    pose proof predecessors_elem_of G _ H1 H2 as H3. apply H0.
+    rewrite SUCC in H3. now apply elem_of_singleton in H3.
+  }
+  assert (EQG: G = {[idA:=A;idB:=B]} ∪ G'). {
+    assert (H: {[idA:=A;idB:=B]} ∪ G' = <[idA:=A]> (<[idB:=B]> G')). {
+      rewrite ?insert_union_singleton_l. symmetry. apply map_union_assoc.
+    }
+    rewrite H.
+    simplify_map_eq. rewrite ?insert_delete; simplify_map_eq; trivial.
+  }
+  rewrite insert_union_singleton_l, EQG. clear EQG.
+  apply denote_ocfg_equiv with (nFROM:={[idA]}) (nTO:={[idB]}); auto; unfold inputs in *.
+    * rewrite dom_insert_L, !dom_singleton_L.
+      replace ({[idA; idB]} ∩ {[idB]}) with ({[idB]}: gset bid) by set_solver.
+      apply disjoint_singleton_l. now apply not_elem_of_singleton.
+    * rewrite dom_insert_L. apply elem_of_subseteq_singleton. set_solver.
+    * rewrite dom_insert_L, !dom_singleton_L.
+      replace ({[idB]} ∖ {[idA; idB]}) with (∅: gset bid) by set_solver.
+      apply empty_subseteq.
+    * rewrite dom_insert_L, !dom_singleton_L. apply elem_of_subseteq_singleton. set_solver.
+    * now apply disjoint_singleton_l.
+    * apply map_disjoint_insert_r. split. now simplify_map_eq.
+      apply map_disjoint_singleton_r. now simplify_map_eq.
+    * apply map_disjoint_singleton_r. apply find_block_none_ocfg_term_rename. now simplify_map_eq.
+    * split; intros id H.
+      + unfold inputs in *. rewrite dom_insert_L in H. rewrite dom_singleton_L in H |- *.
+        subst σ. unfold σfusion. case_match; set_solver.
+      + subst σ. unfold σfusion. assert (id ≠ idA) by now apply not_elem_of_singleton in H. now case_match.
+    * eapply fusion_correct. apply Pattern_BlockFusion_correct. exists G'. split; cycle 1.
+      split. apply EQ. all:trivial. apply INX.
+    * now apply not_elem_of_singleton.
+    * now apply not_elem_of_singleton.
+Qed.
+
+End Theory.
