theories/CCstPDenotation.v
@@ -1,0 +1,141 @@
+(** This file contains the proof of correctness of the Conditional Constant Propagation optimization.
+    It relies on the garantees given by the [CCstP] pattern and on proofs form the [Denotation] file. *)
+
+From Vellvm Require Import Syntax ScopeTheory Semantics Theory Tactics Denotation DenotationTheory.
+From ITree Require Import ITree Eq HeterogeneousRelations.
+From Pattern Require Import Base Patterns Denotation CCstP.
+From Paco Require Import paco.
+From stdpp Require Import prelude fin_maps strings.
+Import List Head Focus Block Patterns gmap Utils.Monads PostConditions Pattern.Denotation ITree.
+
+Definition term_change (t: terminator dtyp) (f: analysis): terminator dtyp := match t with
+  | TERM_Br e l r => match f e with 
+    | One => TERM_Br_1 l
+    | Zero => TERM_Br_1 r
+    | _ => t
+    end
+  | _ => t
+end.
+
+Definition rewrite_term (b: blk) (f: analysis): blk := {|
+  blk_phis       := b.(blk_phis);
+  blk_code       := b.(blk_code);
+  blk_term       := term_change b.(blk_term) f;
+  blk_comments   := b.(blk_comments)
+|}.
+
+Module Type Theory (LP : LLVMParams.LLVMParams).
+Module DE := Denotation.Make LP.
+Import DE.
+Import DT.
+Import DT.D.
+Import LP.
+Import SemNotations.
+Import MonadNotation.
+Import Events.DV.
+
+Variant hidden_cfg  (T: Type) : Type := boxh_cfg (t: T).
+Variant visible_cfg (T: Type) : Type := boxv_cfg (t: T).
+Ltac hide_cfg :=
+  match goal with
+  | h : visible_cfg _ |- _ =>
+      let EQ := fresh "VG" in
+      destruct h as [EQ];
+      apply boxh_cfg in EQ
+  | |- context[denote_ocfg ?cfg _] =>
+      remember cfg as G eqn:VG;
+      apply boxh_cfg in VG
+  end.
+Ltac show_cfg :=
+  match goal with
+  | h: hidden_cfg _ |- _ =>
+      let EQ := fresh "HG" in
+      destruct h as [EQ];
+      apply boxv_cfg in EQ
+  end.
+Notation "'hidden' G" := (hidden_cfg (G = _)) (only printing, at level 10).
+
+
+Module eutt_Notations.
+  Notation "t '======================' '======================' u '======================' '{' R '}'"
+    := (eutt R t u)
+        (only printing, at level 200,
+          format "'//' '//' t '//' '======================' '======================' '//' u '//' '======================' '//' '{' R '}'"
+        ).
+End eutt_Notations.
+Import eutt_Notations.
+
+Definition correct_analysis (f: analysis) := forall t e,
+  (f (t,e) = One -> denote_exp (Some t) e ≈ Ret (UVALUE_I1 VellvmIntegers.Int1.one)) /\
+  (f (t,e) = Zero -> denote_exp (Some t) e ≈ Ret (UVALUE_I1 VellvmIntegers.Int1.zero)).
+
+Lemma rewrite_term_correct {S} f G idB (B: blk) X (P: Pattern S):
+  correct_analysis f -> (idB, B, X) ∈ (MatchAll (CCstP f P) G) ->
+  denote_ocfg_equiv_cond {[idB := B]} {[idB := rewrite_term B f]} ∅ ∅ id.
+Proof.
+  intros AN IN.
+  apply Pattern_CCstP_correct in IN as (G0 & _ & SEM).
+  destruct SEM as [EQ IN (e & l & r & EQt & AN')].
+  unfold denote_ocfg_equiv_cond.
+  einit.
+  ecofix cih.
+  clear cihH.
+  intros fr to _ _.
+  case (decide (to=idB)) as [->|NEQ].
+  - rewrite ?denote_ocfg_in_eq_itree; try by simplify_map_eq.
+    destruct B as [phisB codeB termB cB].
+    remember {| blk_phis := phisB; blk_code := codeB; blk_term := termB; blk_comments := cB |} as B.
+    cbn.
+    setoid_rewrite bind_bind.
+    ebind. econstructor; [reflexivity|]. intros [] ? <-.
+    setoid_rewrite bind_bind. 
+    ebind. econstructor; [reflexivity|]. intros [] ? <-.
+    rewrite !EQt.
+    ebind. econstructor.  { 
+      destruct e as [t e]. pose proof AN t e as [AN1 AN0].
+      destruct AN' as [AN'|AN']; cbn; rewrite AN'; [apply AN0 in AN'|apply AN1 in AN'];
+      rewrite AN', bind_ret_l;cbn; rewrite bind_ret_l; reflexivity.
+    }
+    intros [] ? <-.
+    * etau. ebase. right. apply cihL; set_solver.
+    * eret.
+  - rewrite ?denote_ocfg_nin_eq_itree; now simplify_map_eq.
+Qed.
+
+Theorem Denotation_CCstP_correct {S} f G idB B P (X: S) fr to:
+  correct_analysis f -> (idB, B, X) ∈ (MatchAll (CCstP f P) G) ->
+  ⟦ G ⟧bs (fr, to) ≈ ⟦ <[idB := rewrite_term B f]>(delete idB G) ⟧bs (fr, to).
+Proof.
+  intros AN IN.
+  pose proof IN as IN0.
+  pose proof AN as AN0.
+  apply Pattern_CCstP_correct in IN as (G' & _ & SEM).
+  destruct SEM as [EQ IN (e & l & r & EQt & AN')].
+  pose proof insert_union_singleton_l G' idB (rewrite_term B f) as EQ''.
+  assert (EQ': G = {[idB := B]} ∪ G'). {
+    simplify_map_eq. rewrite <- insert_union_singleton_l. now rewrite insert_delete.
+  } 
+  pose proof ocfg_term_rename_id G' as Hσ.
+  rewrite <- EQ, EQ'', <- Hσ, EQ'.
+  clear EQ'' EQ'.
+  eapply denote_ocfg_equiv.
+  - apply disjoint_empty_r.
+  - apply empty_subseteq.
+  - unfold inputs. rewrite !dom_singleton_L. rewrite difference_diag_L. apply empty_subseteq.
+  - apply empty_subseteq.
+  - apply disjoint_empty_l.
+  - rewrite EQ. apply map_disjoint_insert_r. split. now simplify_map_eq.
+    apply map_disjoint_empty_r.
+  - rewrite Hσ, EQ. apply map_disjoint_insert_r. split. now simplify_map_eq.
+    apply map_disjoint_empty_r.
+  - split.
+    * intros id' IN'. cbn.
+      unfold inputs in *. now rewrite dom_singleton_L in IN' |- *.
+    * now cbn.
+  - eapply rewrite_term_correct; [trivial|apply IN0].
+  - now cbn.
+  - set_solver.
+  - set_solver.
+Qed.
+
+End Theory.
